InferenceInLean/Inference.lean
@@ -38,7 +38,7 @@ structure Proof {sig : Signature} {X : Variables} (Γ : InferenceSystem sig X) w
       simp_all only [List.empty_eq, ne_eq, List.length_eq_zero, not_false_eq_true]
     exact Nat.sub_one_lt hlennonzero) = conclusion
   is_valid : ∀ i (hindex : i < clauses.length), clauses[i] ∈ assumptions ∨
-    ∃ inference ∈ Γ, clauses[i] = inference.conclusion ∧
+    ∃ inference ∈ Γ, clauses[i] = inference.conclusion ∧ inference.condition ∧
       ∀ Clause ∈ inference.premises, ∃ (j : ℕ) (hjindex : j < i), Clause = clauses[j]
 
 @[simp]
@@ -49,7 +49,7 @@ def Provability {sig : Signature} {X : Variables}
 @[simp]
 def Soundness {sig : Signature} {X : Variables} [inst : DecidableEq X]
     (Γ : InferenceSystem sig X) : Prop :=
-  ∀ inference ∈ Γ, ClauseSetEntails inference.premises inference.conclusion
+  ∀ inference ∈ Γ, inference.condition → ClauseSetEntails inference.premises inference.conclusion
 
 @[simp]
 def GeneralSoundness {sig : Signature} {X : Variables} [inst : DecidableEq X]
@@ -70,16 +70,17 @@ theorem generalSoundness_of_soundness {sig : Signature} {X : Variables} [inst : 
       · have hvalid := proof.is_valid (i + 1) hlen
         rcases hvalid with hassump | hconseq
         · simp_all only [Soundness, SetEntails, Assignment, EntailsInterpret]
-        · rcases hconseq with ⟨inference, ⟨hin, ⟨hlast, hprev⟩⟩⟩
+        · rcases hconseq with ⟨inference, ⟨hin, ⟨hlast, hcond, hprev⟩⟩⟩
           rw [hlast]
           have hinfsound := hsound inference hin
           apply hinfsound
-          intro inf_form hprem
-          have hinftrue := hprev inf_form hprem
-          rcases hinftrue with ⟨j, ⟨hjindex, heq⟩⟩
-          have hjtrue := ih j (Nat.le_of_lt_succ hjindex) (Nat.lt_trans hjindex hlen)
-          rw [heq]
-          exact hjtrue
+          · exact hcond
+          · intro inf_form hprem
+            have hinftrue := hprev inf_form hprem
+            rcases hinftrue with ⟨j, ⟨hjindex, heq⟩⟩
+            have hjtrue := ih j (Nat.le_of_lt_succ hjindex) (Nat.lt_trans hjindex hlen)
+            rw [heq]
+            exact hjtrue
     intro F hF
     have hfindex : ∃ (i : ℕ) (hindex : i < proof.clauses.length), proof.clauses[i] = F :=
       List.mem_iff_getElem.mp hF
@@ -98,12 +99,13 @@ theorem generalSoundness_of_soundness {sig : Signature} {X : Variables} [inst : 
   · subst hassumptions hconclusion
     obtain ⟨inference, h⟩ := hr
     obtain ⟨hinf, right⟩ := h
-    obtain ⟨hconcs, hforms⟩ := right
+    obtain ⟨hconcs, hcond, hforms⟩ := right
     have h := hsound inference hinf
     rw [hconcs]
     apply h
-    intro G hgprem
-    have hinf := hforms G hgprem
-    rcases hinf with ⟨j, hjnotconc, hginforms⟩
-    simp_all only [Soundness, SetEntails, Assignment, EntailsInterpret,
-      implies_true, List.getElem_mem]
+    · exact hcond
+    · intro G hgprem
+      have hinf := hforms G hgprem
+      rcases hinf with ⟨j, hjnotconc, hginforms⟩
+      simp_all only [Soundness, SetEntails, Assignment, EntailsInterpret,
+        implies_true, List.getElem_mem]
